SeparationLogic/algorithms/Tarjan_directed/Tarjan_scc_low_defs.v
@@ -74,6 +74,16 @@ Section LOW_DEFS.
   Definition done_reachable_closed (done: V -> Prop) (s: @SCCSt V): Prop :=
     forall v w, done v -> ~ In v (stack s) -> dg_reachable g v w -> w ∈ visited s.
 
+  Definition done_tree_reachable_closed
+             (u: V) (done: V -> Prop) (s: @SCCSt V): Prop :=
+    forall v w,
+      done v ->
+      ~ In v (stack s) ->
+      fa s v = u ->
+      fa s v <> v ->
+      dg_reachable g v w ->
+      w ∈ visited s.
+
   Definition fa_child_of_u (u: V) (s: @SCCSt V): Prop :=
     forall v, fa s v = u /\ fa s v <> v -> dg_step g u v.
 
@@ -109,6 +119,7 @@ Section LOW_DEFS.
     In u (stack s) /\
     done_visited done s /\
     done_reachable_closed done s /\
+    done_tree_reachable_closed u done s /\
     low_frontier u done s /\
     low_src u done s /\
     children_low_valid u done s /\
